Add an intermediate cleanup step for cost functions
There is now an intermediate cost function, which is equal to the uncleaned-one,
but where the superfluous ceil have been removed. It is still possibly less
simple than the fully cleaned cost function (which only dominates the uncleaned
cost function), but can be used to prove the monotonicity subgoal.

examples/proofs/CFMLBigO.v
@@ -128,34 +128,39 @@ Record specO
       cost_dominated : dominated A cost bound
     }.
 
-Definition cleanup_cost (A : filterType) (cost cost_clean : A -> Z) :=
-  dominated A cost cost_clean.
+Definition cleanup_cost (A : filterType) (cost cost_clean_eq cost_clean : A -> Z) :=
+  (forall (x : A), cost x = cost_clean_eq x) /\
+  dominated A cost_clean_eq cost_clean.
 
 Lemma specO_refine_prove :
   forall (A : filterType) (le : A -> A -> Prop)
-         (cost cost_clean bound : A -> Z)
+         (cost cost_clean_eq cost_clean bound : A -> Z)
          (spec : (A -> Z) -> Prop),
     spec cost ->
-    cleanup_cost A cost cost_clean ->
+    cleanup_cost A cost cost_clean_eq cost_clean ->
     (forall x, 0 <= cost x) ->
-    monotonic le Z.le cost ->
+    monotonic le Z.le cost_clean_eq ->
     dominated A cost_clean bound ->
     specO A le spec bound.
 Proof.
-  intros ? le cost cost_clean bound.
+  intros ? le cost cost_clean_eq cost_clean bound.
   introv S D1 N M D2.
   econstructor; eauto.
-  rewrite D1. assumption.
+  - apply Monotonic.monotonic_eq with cost_clean_eq; auto.
+    intro. rewrite~ (proj1 D1).
+  - apply dominated_eq_l with cost_clean_eq.
+    rewrite~ (proj2 D1). intro. rewrite~ (proj1 D1).
 Qed.
 
 Ltac xspecO_refine_base cost_name :=
   match goal with
     |- specO ?A ?le _ _ =>
+    let cost_clean_eq := fresh "cost_clean_eq" in
     let cost_clean := fresh "cost_clean" in
     refine (let cost_name := (fun (x : A) => ceil _ ) : A -> Z in _);
-    evar (cost_clean : A -> Z);
-    eapply (@specO_refine_prove A le cost_name cost_clean);
-    subst cost_clean;
+    evar (cost_clean : A -> Z); evar (cost_clean_eq : A -> Z);
+    eapply (@specO_refine_prove A le cost_name cost_clean_eq cost_clean);
+    subst cost_clean cost_clean_eq;
     [ unfold cost_name | | intro; apply ceil_pos
       | subst cost_name | subst cost_name ]
   end.
@@ -202,15 +207,40 @@ Ltac hide_evars_then cont :=
     cont tt
   end.
 
+Ltac clean_ceil_math :=
+  try cases_if; auto with zarith.
+
+(* Simple tactic to eliminate occurences of [ceil x] when x is proved
+   nonnegative by [clean_ceil_math].
+*)
+Ltac clean_ceil :=
+   repeat match goal with
+   | |- context[ ceil ?x ] => rewrite (@ceil_eq x) by clean_ceil_math
+   end.
+
 Ltac simple_cleanup_cost :=
-  intro; simpl; hide_evars_then ltac:(fun _ => ring_simplify).
+  simpl; hide_evars_then ltac:(fun _ => ring_simplify).
+
+Ltac simple_cleanup_cost_eq :=
+  simpl; clean_ceil; simple_cleanup_cost.
+
+Ltac unfold_cost_lhs :=
+  match goal with
+  | |- ?cost ?x = ?rhs => unfold cost
+  end.
 
 Ltac cleanup_cost :=
   unfold cleanup_cost;
-  eapply dominated_eq_r;
-  [ dominated_cleanup_cost |];
-  simple_cleanup_cost;
-  reflexivity.
+  split; [
+    intro; unfold_cost_lhs;
+    simple_cleanup_cost_eq;
+    reflexivity
+  | eapply dominated_eq_r;
+    [ dominated_cleanup_cost |];
+    intro;
+    simple_cleanup_cost;
+    reflexivity
+  ].
 
 
 (* Custom CF rules and tactics ************************************************)
